LeanScratch/Semantics/PCF/Denote.lean
@@ -1,0 +1,58 @@
+import LeanScratch.Semantics.PCF.Stx
+import LeanScratch.Semantics.PCF.Red
+import LeanScratch.Domain.Basic
+
+open Dom
+
+namespace PCF
+
+noncomputable def Ty.denote : Ty → Sigma Dom
+  | .nat => ⟨Flat Nat, by infer_instance⟩
+  | .bool => ⟨Flat Bool, by infer_instance⟩
+  | .arrow a b =>
+    have ⟨a, ha⟩ := a.denote
+    have ⟨b, hb⟩ := b.denote
+    ⟨CFunc a b, by infer_instance⟩
+
+noncomputable def context : List Ty → Sigma Dom
+  | [] => ⟨Unit, by infer_instance⟩
+  | hd :: tl =>
+    have ⟨dtl, htl⟩ := context tl
+    have ⟨dhd, hhd⟩ := hd.denote
+    ⟨dhd × dtl, by infer_instance⟩
+
+namespace Expr
+def succ.denote' : Flat Nat → Flat Nat
+  | .obj v => .obj v.succ
+  | .bot => .bot
+
+noncomputable instance succ.denote'.cont : Continous.Helper (succ.denote') where
+  mono
+    | .obj a, .obj _, .obj_obj => .obj_obj
+    | .bot, .obj b, h => .bot_obj
+    | .bot, .bot, h => .bot_bot
+  preserves_lubs c hc := by
+    dsimp [complete]
+    have ⟨f, .intro⟩ := Flat.finite c hc
+    sorry
+
+def succ.denote : CFunc (Flat Nat) (Flat Nat) where
+  f := succ.denote'
+  continous := succ.denote'.cont 
+
+def pred.denote : Flat Nat → Flat Nat
+  | .obj (.succ v) => .obj v
+  | .obj 0 => .bot
+  | .bot => .bot
+
+def z?.denote : Flat Nat → Flat Bool
+  | .obj (.succ _) => .obj .false
+  | .obj 0 => .obj .true
+  | .bot => .bot
+
+def bvar.denote : {Γ : _} → (v : Fin2 Γ.length) → (context Γ).fst → (Γ.getFin2 v).denote.fst
+  | _ :: _, .fz, ⟨o, _⟩ => o
+  | _ :: _, .fs v, ⟨_, t⟩ => bvar.denote v t
+
+#check CFunc.mp
+
