LeanScratch/Semantics/PCF/Red.lean
@@ -1,0 +1,73 @@
+import LeanScratch.Semantics.PCF.Stx
+/- import LeanScratch.Semantics.PCF.Typed -/
+import Mathlib.Data.Rel
+import Mathlib.Data.List.AList
+import LeanScratch.Relation
+
+namespace PCF
+
+inductive Red : Expr [] τ → Expr [] τ → Prop
+  | val : v.IsValue → Red v v
+  | succ :
+    Red t v
+    → Red t.succ v.succ
+  | pred :
+    Red t v.succ
+    → Red t.pred v
+  | z?zero :
+    Red t .zero
+    → Red t.z? .tt
+  | z?succ : Red t (.succ v)
+    → Red t.z? .ff
+  | eif_tt : Red c .tt
+    → Red t v
+    → Red (c.eif t f) v
+  | eif_ff : Red c .ff
+    → Red f v
+    → Red (c.eif t f) v
+  | abs_cbn /- (en : Cbn) -/ :
+    {t : Expr [] $ .arrow arg o}
+    → Red t (.abs arg t')
+    → Red (t'.β u) v
+    → Red (.app t u) v
+  | fix : Red (.app t t.fix) v
+    → Red t.fix v
+
+theorem Red.res_val (h : Red e v) : v.IsValue := by
+  induction h
+  any_goals solve_by_elim
+  case pred ih =>
+    cases ih; assumption
+
+theorem Red.val_hold (hV : e.IsValue) (h : Red e v) : e = v := by
+  induction hV <;> cases h
+  any_goals rfl
+  case succ ih _ h => rw [ih h]
+
+theorem Red.confluent (ha : Red e v₁) (hb : Red e v₂) : v₁ = v₂ := by
+  induction ha
+  case val ih => exact Red.val_hold ih hb
+  all_goals cases hb
+  any_goals solve_by_elim
+  any_goals (rename_i hv; cases hv; done)
+  case succ.val h _ hv =>
+    cases hv; rename_i hv
+    rw [Red.val_hold hv h]
+  case pred.pred ih h=> exact (Expr.succ.injEq _ _).mp $ ih h
+  case z?zero.z?succ ih _ h => exact Expr.noConfusion $ ih h
+  case z?succ.z?zero ih h => exact Expr.noConfusion $ ih h
+  case eif_tt.eif_ff ih _ h _=> exact Expr.noConfusion $ ih h
+  case eif_ff.eif_tt ih _ h _=> exact Expr.noConfusion $ ih h
+  case abs_cbn.abs_cbn ihf iha _ hf ha =>
+    obtain rfl := Expr.abs.inj $ ihf hf
+    exact iha ha
+
+def Context (τ : Ty) : Type := Sigma $ Expr [τ]
+
+def ContEquiv (a b : Expr [] τ) : Prop := ∀ c : Context τ,
+  ∀ v, Red (c.snd.β a) v ↔ Red (c.snd.β b) v
+
+theorem ContEquiv.eqIn : ContEquiv a a := fun _ _ => Eq.to_iff rfl
+
+
+
