LeanScratch/Semantics/PCF/Stx.lean
@@ -1,0 +1,113 @@
+import Mathlib.Data.Rel
+import Mathlib.Data.Finset.Basic
+import Mathlib.Tactic.Linarith.Frontend
+import LeanScratch.Fin2
+
+namespace PCF
+
+inductive Ty
+  | bool
+  | nat
+  | arrow (arg res : Ty)
+deriving DecidableEq, Repr
+
+inductive Expr : List Ty → Ty → Type
+  | zero : Expr Γ .nat
+  | succ (e : Expr Γ .nat) : Expr Γ .nat
+  | pred (e : Expr Γ .nat) : Expr Γ .nat
+
+  | tt : Expr Γ .bool
+  | ff : Expr Γ .bool
+  | z? (e : Expr Γ .nat) : Expr Γ .bool
+
+  | eif (cond : Expr Γ .bool) (t f : Expr Γ τ) : Expr Γ τ
+
+  | bvar idx : Expr Γ (Γ.getFin2 idx)
+  | abs (ty : Ty) (body : Expr (ty :: Γ) ret) : Expr Γ (.arrow ty ret)
+  | app (fn : Expr Γ (.arrow arg ret)) (arg : Expr Γ arg) : Expr Γ ret
+  | fix (e : Expr Γ (.arrow τ τ)) : Expr Γ τ
+deriving Repr
+
+namespace Expr
+
+inductive IsValue : Expr Γ τ → Prop
+  | tt : IsValue .tt
+  | ff : IsValue .ff
+  | zero : IsValue .zero
+  | succ : IsValue a → IsValue (.succ a)
+  | fn : IsValue (.abs ty body)
+
+def extend {c : List α} : {a b : List α} → Fin2 (a ++ c).length → Fin2 (a ++ b ++ c).length
+  | [], [], x => x
+  | [], _ :: tb, v => .fs $ extend v
+  | _ :: ta, b, .fz => .fz
+  | _ :: ta, b, .fs v => .fs $ extend v
+
+theorem extend.eq {c : List α}
+    : {a b : List α}
+    → {i : Fin2 (a ++ c).length}
+    → (a ++ c).getFin2 i = (a ++ b ++ c).getFin2 (@extend _ c a b i) := by
+  intro a b i
+  induction a, b, i using extend.induct
+  <;> unfold extend
+  any_goals rfl
+  all_goals assumption
+
+def bvarShift : Expr (Γskip ++ Γ₁) τ → Expr (Γskip ++ Γshift ++ Γ₁) τ
+  | .bvar n =>
+    cast (congr rfl extend.eq.symm) $ .bvar (extend n)
+  | .abs ty body => .abs ty (body.bvarShift (Γskip := ty :: Γskip))
+  | .app a b => .app a.bvarShift b.bvarShift
+  | .eif c t f => .eif c.bvarShift t.bvarShift f.bvarShift
+  | .succ v => .succ v.bvarShift
+  | .pred v => .pred v.bvarShift
+  | .fix v => .fix v.bvarShift
+  | .z? v => .z? v.bvarShift
+  | .tt => .tt
+  | .ff => .ff
+  | .zero => .zero
+
+def bvarShift' : Expr Γ₁ τ → Expr (Γshift ++ Γ₁) τ := bvarShift (Γskip := [])
+
+/- def replace.bvar (bvarId idx_shift : ℕ) (replace : Expr) : Expr _ τ := -/
+/-   match compare bvarId idx_shift with -/
+/-   | .lt => .bvar bvarId -/
+/-   | .eq => replace.bvarShift idx_shift 0 -/
+/-   | .gt => .bvar bvarId.pred -/
+
+def replace.bvar (repl : Expr Γ τ)
+    (ΓPre : List _)
+    : (Γctx : List _)
+    → (n : Fin2 (Γctx ++ [τ] ++ Γ).length)
+    → Expr (ΓPre ++ Γctx ++ Γ) ((Γctx ++ [τ] ++ Γ).getFin2 n)
+  | [], .fz =>
+    have := bvarShift' (Γshift := ΓPre) repl
+    cast (congr (congr rfl (congr (congr rfl (List.append_nil _).symm) rfl)) rfl) this
+  | [], .fs v =>
+    have := bvarShift' (Γshift := ΓPre) $ .bvar (Γ := Γ) v
+    cast (congr (congr rfl (List.append_assoc _ _ _).symm) rfl) this
+  | hd :: tl, .fz =>
+    have := bvarShift' (Γshift := ΓPre)
+      $ Expr.bvar (Γ := hd :: tl ++ Γ) (.fz (n := (tl ++ Γ).length))
+    cast (congr (congr rfl (List.append_assoc _ _ _).symm) rfl) this
+  | hd :: tl, .fs v =>
+    have := replace.bvar repl (ΓPre ++ [hd]) tl v
+    cast (by congr 2; exact (List.append_cons _ _ _).symm) this
+
+def replace (body : Expr (Γctx ++ [τ] ++ Γ) τo) (repl : Expr Γ τ) : Expr (Γctx ++ Γ) τo := match body with
+  | .bvar n => replace.bvar repl [] Γctx n
+  | .abs ty body => .abs ty (body.replace (Γctx := ty :: Γctx) repl)
+
+  | .app a b => .app (a.replace repl) (b.replace repl)
+  | .eif c t f => .eif (c.replace repl) (t.replace repl) (f.replace repl)
+  | .succ v => .succ (v.replace repl)
+  | .pred v => .pred (v.replace repl)
+  | .fix v => .fix (v.replace repl)
+  | .z? v => .z? (v.replace repl)
+
+  | .tt => .tt
+  | .ff => .ff
+  | .zero => .zero
+
+def β : Expr (τ :: Γ) τo → Expr Γ τ → Expr Γ τo := replace (Γctx := [])
+
