LeanScratch/Semantics/PCF/TC.lean
@@ -1,0 +1,17 @@
+import LeanScratch.Semantics.PCF.Red
+import LeanScratch.Computation.GRFs
+
+namespace PCF
+
+def GRFType : Nat → Ty
+  | 0 => .nat
+  | n+1 => .arrow .nat $ GRFType n
+
+-- TODO
+def translate : Comp.GRFunStx Unit n → Expr
+  | .comp _ _ => sorry
+  | .mini _ _ => sorry
+  | .succ => sorry
+  | .zero => sorry
+  | .proj _ => sorry
+  | .nRec _ _ => sorry
