LeanScratch/Subsingleton.lean
@@ -1,0 +1,6 @@
+
+def Subsingleton.neg (t : Type _) : Type _ := (v : t) → Empty
+
+instance : Subsingleton (Subsingleton.neg t) where
+  allEq a b := funext λ i ↦ Subsingleton.allEq (a i) (b i)
+
